defined under_ctx

lawyer/nonblocking/wfree_traces.v
@@ -9,17 +9,106 @@ Close Scope Z.
 
 Section UnderCtx.
 
-  (* TODO: move *)
-  Definition under_ctx (K: ectx heap_lang) (e: expr): option expr.
-  Admitted.
+  Local Definition check P `{Decision P} (e: expr) :=
+    if (decide P) then Some e else None. 
+
+  Definition under_ctx_item (Ki: ectx_item) (e: expr): option expr :=
+    match Ki, e with 
+  | AppLCtx vc2, App e e2 => check (e2 = of_val vc2) e
+  | AppRCtx ec1, App e1 e => check (e1 = ec1) e
+  | UnOpCtx opc, UnOp op e => check (op = opc) e
+  | BinOpLCtx opc vc, BinOp op e1 v2 => check (op = opc /\ v2 = vc) e1
+  | BinOpRCtx opc ec, BinOp op e1 e2 => check (op = opc /\ e1 = ec) e2
+  | IfCtx ec1 ec2, If e e1 e2 => check (e1 = ec1 /\ e2 = ec2) e
+  | PairLCtx vc2, Pair e (Val v2) => check (v2 = vc2) e
+  | PairRCtx ec1, Pair e1 e => check (e1 = ec1) e
+  | FstCtx, Fst e => Some e
+  | SndCtx, Snd e => Some e
+  | InjLCtx, InjL e => Some e
+  | InjRCtx, InjR e => Some e
+  | CaseCtx ec1 ec2, Case e e1 e2 => check (e1 = ec1 /\ e2 = ec2) e
+  | AllocNLCtx vc2, AllocN e (Val v2) => check (v2 = vc2) e
+  | AllocNRCtx ec1, AllocN e1 e => check (e1 = ec1) e
+  | LoadCtx, Load e => Some e
+  | StoreLCtx vc2, Store e (Val v2) => check (v2 = vc2) e
+  | StoreRCtx ec1, Store e1 e => check (e1 = ec1) e
+  | CmpXchgLCtx vc1 vc2, CmpXchg e (Val v1) (Val v2) => check (v1 = vc1 /\ v2 = vc2) e
+  | CmpXchgMCtx ec0 vc2, CmpXchg e0 e (Val v2) => check (e0 = ec0 /\ v2 = vc2) e
+  | CmpXchgRCtx ec0 ec1, CmpXchg e0 e1 e => check (e0 = ec0 /\ e1 = ec1) e
+  | FaaLCtx vc2, FAA e (Val v2) => check (v2 = vc2) e
+  | FaaRCtx ec1, FAA e1 e => check (e1 = ec1) e
+  | _, _ => None
+    end.
+
+  Local Lemma not_eq_helper (x e1 e2: expr)
+    (NEQ: e1 ≠ e2):
+    None = Some x <-> e1 = e2.
+  Proof using. trans False; done. Qed.
+    
+  Lemma under_ctx_item_spec Ki e e':
+    under_ctx_item Ki e = Some e' <-> fill_item Ki e' = e.
+  Proof using.
+    destruct Ki, e; simpl.
+    all: try by apply not_eq_helper. 
+    Local Ltac solve_iff := rewrite /check; destruct decide; try apply not_eq_helper; subst; set_solver.
+    all: try by solve_iff.
+    all: try by set_solver. 
+    - destruct e2; by apply not_eq_helper || solve_iff.
+    - destruct e2; by apply not_eq_helper || solve_iff.
+    - destruct e2; by apply not_eq_helper || solve_iff.
+    - destruct e2, e3; by apply not_eq_helper || solve_iff.
+    - destruct e3; by apply not_eq_helper || solve_iff.
+    - destruct e2; by apply not_eq_helper || solve_iff.
+  Qed. 
+
+  Fixpoint under_ctx (K: ectx heap_lang) (e: expr): option expr :=
+    match K with
+    | [] => Some e
+    | Ki :: K' => from_option (under_ctx_item Ki) None (under_ctx K' e)
+    end. 
 
   Lemma under_ctx_spec K e e':
-    under_ctx K e = Some e' <-> ectx_fill K e' = e.
-  Proof using. Admitted.
+    under_ctx K e = Some e' <-> fill K e' = e.
+  Proof using.
+    generalize dependent e. generalize dependent e'.
+    induction K.
+    { simpl. set_solver. }
+    intros. simpl. destruct under_ctx eqn:ITEM.
+    2: { apply not_eq_helper.
+         intros EQ. rewrite -IHK in EQ. congruence. }
+    rewrite under_ctx_item_spec.
+    apply IHK in ITEM. simpl in *.
+    rewrite -ITEM. split.
+    + by intros <-.
+    + by intros ?%ectx_fill_inj.
+  Qed.
+
+  Lemma under_ctx_spec_neg K e:
+    under_ctx K e = None <-> forall e', fill K e' ≠ e.
+  Proof using.
+    simpl. split; intros. 
+    - intros EQ%under_ctx_spec. congruence.
+    - destruct under_ctx eqn:UC; [| done].
+      apply under_ctx_spec in UC.
+      edestruct H; eauto.
+  Qed.
 
   Lemma under_ctx_fill K e:
-    under_ctx K (ectx_fill K e) = Some e.
-  Proof using. Admitted. 
+    under_ctx K (fill K e) = Some e.
+  Proof using. by apply under_ctx_spec. Qed.
+
+  Lemma under_ctx_val_Some_inv (e ec: expr) K
+    (CTX: under_ctx K e = Some ec)
+    (VAL: is_Some (language.to_val e)):
+    K = ectx_emp /\ ec = e.
+  Proof using.
+    apply under_ctx_spec in CTX. simpl in *.
+    destruct K; simpl in CTX; subst; try done.
+    simpl in VAL.
+    rewrite fill_not_val in VAL.
+    { by destruct VAL. }
+    by destruct e0. 
+  Qed.
 
 End UnderCtx.
 
